\documentclass{article}

\usepackage{geometry}
\usepackage{graphicx}
\usepackage{subfigure}
\usepackage{diagbox}
\usepackage{amsthm}
\newtheorem{theorem}{Theorem}[section]
\newtheorem{lemma}[theorem]{Lemma} 
\geometry{a4paper,left=2cm,right=2cm,top=1cm,bottom=1cm}

\title{Stochastic Galerkin Method}
\author{Yikai Wang}
\date{\today}

\begin{document}
\maketitle

\section{General Procedure}

\subsection{Problem}
\[ -\nabla\cdot(a(\omega,x)\nabla u(\omega,x))=f(\omega,x)  \ (\omega,x)\in \Omega \times D\]
\[u(\omega,x)= 0 \ x \in \partial D\]
\subsection{Tensor Product}
\[ (f\otimes g)(x,y)=f(x)g(y) \]
\[ ((A\otimes B)_{i_1 j_1})_{i_2 j_2} = A_{i_1 j_1}B_{i_2 j_2} \]
\subsection{Solution}
\[\mathbf{E}[\int_{D}a\nabla u \nabla v dx]=E[\int_{D}fvdx] \]
\[v(x) = \sum_{i=1}^{N}V_i \phi_i(x) \]
\[ \int_{D}a \nabla(\sum_{i=1}^{N}U_i \phi_i(x))\cdot \nabla \phi_jdx = \int_{D}f\phi_jdx \]
\[\sum_{i=1}^{N}U_i \int_{D}a\nabla \phi_i \cdot \nabla \phi_j dx = \int_{D}f\phi_j dx \]
\[KU = F\]
\[a(\omega,x) = \bar{a}+\sum_{l=1}^{\infty}\varphi_l(x)y_l(\omega) \]
\[u(\omega,x) = \sum_{n=1}^{Q}\sum_{i=1}^{N}(U_n)_{i}\psi_n(\omega)\phi_i(x) \]
\[\mathbf{E}[\int_{D}a \nabla \sum_{i=1}^{N}\sum_{n=1}^{Q}(U_n)_i \psi_n \phi_i \cdot \nabla\psi_m \phi_j dx] = \mathbf{E}[\int_{D}f\psi_m \phi_j dx] \]
\[\sum_{i=1}^{N}\sum_{n=1}^{Q}(U_n)_i \mathbf{E}[\int_{D}a\nabla \psi_n \phi_i \cdot \nabla \psi_m \phi_j dx=\mathbf{E}[\int_{D}f\psi_m \phi_j dx] \]
\[\sum_{i=1}^{N}\sum_{n=1}^{Q}(U_n)_i \mathbf{E}[\psi_n \psi_m \int_{D}a\nabla \phi_i \cdot \nabla\phi_j dx] = \mathbf{E}[\psi_m \int_{D}f\phi_j dx] \]
\[a(\omega,x)=\sum_{l=0}^{S}a_l(x)y_l(\omega) \]
\[\sum_{l=0}^{S}\sum_{i=1}^{N}\sum_{n=1}^{Q}(U_n)_i \mathbf{E}[y_l \psi_n \psi_m \int_{D}a_l \nabla \phi_i \cdot \nabla\phi_j dx] =\mathbf{E}[\psi_m \int_{D}f\phi_j dx] \]
\[\sum_{l=0}^{S}\sum_{i=1}^{N}\sum_{n=1}^{Q}(U_n)_i \mathbf{E}[y_l \psi_n \psi_m]\int_{D}a_l \nabla \phi_i \cdot \nabla\phi_j dx =\mathbf{E}[\psi_m \int_{D}f\phi_j dx]\]
\[\sum_{l=0}^{S}\sum_{i=1}^{N}\sum_{n=1}^{Q}(U_n)_i(G_l)_{nm}(K_l)_{ij} = (F_m)_j \]
\[\sum_{l=0}^{S}\sum_{i=1}^{N}\sum_{n=1}^{Q}(U_n)_i((G_l \otimes K_l)_{nm})_{ij} = (F_m)_j \]
\[\sum_{l=0}^{S}(G_l \otimes K_l)U = F \]

\end{document}